stdpp/fin_map_dom.v
@@ -284,21 +284,25 @@ Proof.
   intros a. rewrite !elem_of_dom. intros [c Hm].
   apply lookup_omap_Some in Hm. naive_solver.
 Qed.
+
 Lemma map_compose_dom_subseteq {C} `{FinMap K' M'} (m: M' C) (n : M K') :
   dom (m ∘ₘ n : M C) ⊆@{D} dom n.
 Proof. apply dom_omap_subseteq. Qed.
-Lemma map_compose_min_r_dom {C} `{FinMap K' M', !RelDecision (∈@{D})} (m : M C) (n : M' K) :
-  m ∘ₘ n = m ∘ₘ (filter (λ '(_,b), b ∈ dom m) n).
+Lemma map_compose_min_r_dom {C} `{FinMap K' M', !RelDecision (∈@{D})}
+    (m : M C) (n : M' K) :
+  m ∘ₘ n = m ∘ₘ filter (λ '(_,b), b ∈ dom m) n.
 Proof.
   rewrite map_compose_min_r. f_equal.
   apply map_filter_ext. intros. by rewrite elem_of_dom.
 Qed.
 
-Lemma map_compose_empty_iff_dom_img {C} `{FinMap K' M', !RelDecision (∈@{D})} (m : M C) (n : M' K) :
+Lemma map_compose_empty_iff_dom_img {C} `{FinMap K' M', !RelDecision (∈@{D})}
+    (m : M C) (n : M' K) :
   m ∘ₘ n = ∅ ↔ dom m ## map_img n.
 Proof.
-  rewrite map_compose_empty_iff. set_unfold.
-  setoid_rewrite elem_of_dom. by setoid_rewrite elem_of_map_img.
+  rewrite map_compose_empty_iff, elem_of_disjoint.
+  setoid_rewrite elem_of_dom. setoid_rewrite eq_None_not_Some.
+  setoid_rewrite elem_of_map_img. naive_solver.
 Qed.
 
 (** If [D] has Leibniz equality, we can show an even stronger result.  This is a
